theories/Dot/unary_lr.v
@@ -48,11 +48,11 @@ Section logrel.
     ev; simplify_eq. by iApply (leadsto_agree _ interp1 interp2).
   Qed.
 
-  Lemma dm_to_type_intro s σ φ : s ↝ φ -∗ dtysem σ s ↗ φ (to_subst σ).
+  Lemma dm_to_type_intro d s σ φ :
+    d = dtysem σ s → s ↝ φ -∗ d ↗ φ (to_subst σ).
   Proof. iIntros. iExists s, σ , φ. by iSplit. Qed.
 
-  Global Arguments dm_to_type : simpl never.
-  (* Global Opaque dm_to_type. *)
+  Global Opaque dm_to_type.
 
   Definition def_interp_tmem interp1 interp2 : envPred dm Σ :=
     λ ρ d,
